\documentclass{article}
\usepackage{graphicx} % Required for inserting images
\usepackage{amsmath}
\title{\vspace{-3.5cm}Homework for Linear Algebra\\September 20,2024}
\author{Chengyu Zhang}
\date{}
\begin{document}



\maketitle
\paragraph{Exercise 1.}
1.(i)$\rightarrow$(ii) Using the definition of f from (i):
\[
f(x_1+x_2)=a(x_1+x_2)=ax_1+ax_2=f(x_1)+f(x_2)
\]
\[f(cx)=acx=cf(x)\]
\\2.(ii)$\rightarrow$(i) When $x=0$ , using additivity : \[f(0)=2f(0)=0\]\\
When $x \neq 0$ , using multiplication : \[f(x)=f(x*1)=x*f(1)\]\\
So,when a=f(1), we have $f(x)=ax$

\paragraph{Exercise 2}
(a)line (b)plane  (c)all of $R^3$


\paragraph{Exercise 3.} $c=3$ and $d = 9$\\
(3,3,6) isn't on the plane consisting of $\boldsymbol{v}$ and $\boldsymbol{w}$.

\paragraph{Exercise 4.}Taking a small scale as an example,assume
\[
A=\begin{bmatrix}
a_{11} & a_{12}\\
a_{21} & a_{22}\\
\end{bmatrix}
 B=\begin{bmatrix}
b_{11} & b_{12}\\
b_{21} & b_{22}\\
\end{bmatrix}
 C=\begin{bmatrix}
c_{11} & c_{12}\\
c_{21} & c_{22}\\
\end{bmatrix}
\]
(i)\[A+B=
\begin{bmatrix}
a_{11}+b_{11} & a_{12}+b_{12}\\
a_{21}+b_{21} & a_{22}+b_{22}\\
\end{bmatrix}
= B+A\] \\
(ii)\[c(A+B)=
\begin{bmatrix}
c(a_{11}+b_{11}) & c (a_{12}+b_{12})\\
c(a_{21}+b_{21}) & c(a_{22}+b_{22})\\
\end{bmatrix}\\=
\begin{bmatrix}
ca_{11}+cb_{11} & ca_{12}+cb_{12}\\
ca_{21}+cb_{21} & ca_{22}+cb_{22}\\
\end{bmatrix}
=cA+cB\] \\
(iii)\[
A+(B+C)=
\begin{bmatrix}
a_{11} & a_{12}\\
a_{21} & a_{22}\\
\end{bmatrix}
+
\begin{bmatrix}
b_{11}+c_{11} & b_{12}+c_{12}\\
b_{21}+c_{21} & b_{22}+c_{22}\\
\end{bmatrix}
=
\begin{bmatrix}
a_{11}+b_{11}+c_{11} & a_{12}+b_{12}+c_{12}\\
a_{21}+b_{21}+c_{21} & a_{22}+b_{22}+c_{22}\\
\end{bmatrix} 
\]\\
\[
(A+B)+C=
\begin{bmatrix}
a_{11}+b_{11} & a_{12}+b_{12}\\
a_{21}+b_{21} & a_{22}+b_{22}\\
\end{bmatrix}
+
\begin{bmatrix}
c_{11} & c_{12}\\
c_{21} & c_{22}\\
\end{bmatrix}
=A+(B+C)
\]\\
(iv)
\[
A(B+C)=
\begin{bmatrix}
a_{11} & a_{12}\\
a_{21} & a_{22}\\
\end{bmatrix}
\begin{bmatrix}
b_{11}+c_{11} & b_{12}+c_{12}\\
b_{21}+c_{21} & b_{22}+c_{22}\\
\end{bmatrix}
\]
\[
=
\begin{bmatrix}
a_{11}(b_{11} + c_{11}) + a_{12}(b_{21} + c_{21}) & a_{11}(b_{12} + c_{12}) + a_{12}(b_{22} + c_{22}) \\
a_{21}(b_{11} + c_{11}) + a_{22}(b_{21} + c_{21}) & a_{21}(b_{12} + c_{12}) + a_{22}(b_{22} + c_{22}) \\
\end{bmatrix}
\]
\[
=
\begin{bmatrix}
a_{11}b_{11} + a_{12}b_{21} & a_{11}b_{12} + a_{12}b_{22} \\
a_{21}b_{11}+ a_{22}b_{21}& a_{21}b_{12} + a_{22}b_{22} \\
\end{bmatrix}
+
\begin{bmatrix}
a_{11}c_{11} + a_{12}c_{21} & a_{11}c_{12} + a_{12}c_{22} \\
a_{21}c_{11}+ a_{22}c_{21}& a_{21}c_{12} + a_{22}c_{22} \\
\end{bmatrix}
=AB+AC
\]
\\(v)
\[
(A+B)C =
\begin{bmatrix}
a_{11} + b_{11} & a_{12} + b_{12} \\
a_{21} + b_{21} & a_{22} + b_{22} \\
\end{bmatrix}
\begin{bmatrix}
c_{11} & c_{12} \\
c_{21} & c_{22} \\
\end{bmatrix}
\]
\[
=
\begin{bmatrix}
(a_{11} + b_{11})c_{11} + (a_{12} + b_{12})c_{21} & (a_{11} + b_{11})c_{12} + (a_{12} + b_{12})c_{22} \\
(a_{21} + b_{21})c_{11} + (a_{22} + b_{22})c_{21} & (a_{21} + b_{21})c_{12} + (a_{22} + b_{22})c_{22} \\
\end{bmatrix}
\]
\[
=
\begin{bmatrix}
a_{11}c_{11} + a_{12}c_{21} & a_{11}c_{12} + a_{12}c_{22} \\
a_{21}c_{11}+ a_{22}c_{21}& a_{21}c_{12} + a_{22}c_{22} \\
\end{bmatrix}
+
\begin{bmatrix}
b_{11}c_{11} + b_{12}c_{21} & b_{11}c_{12} + b_{12}c_{22} \\
b_{21}c_{11}+ b_{22}c_{21}& b_{21}c_{12} + b_{22}c_{22} \\
\end{bmatrix}
=AC+BC
\]
\\(vi)
\[
A(BC) =
\begin{bmatrix}
a_{11} & a_{12} \\
a_{21} & a_{22} \\
\end{bmatrix}
\begin{bmatrix}
b_{11}c_{11} + b_{12}c_{21} & b_{11}c_{12} + b_{12}c_{22} \\
b_{21}c_{11} + b_{22}c_{21} & b_{21}c_{12} + b_{22}c_{22} \\
\end{bmatrix}
\]
\[
=
\begin{bmatrix}
a_{11}(b_{11}c_{11} + b_{12}c_{21}) + a_{12}(b_{21}c_{11} + b_{22}c_{21}) & a_{11}(b_{11}c_{12} + b_{12}c_{22}) + a_{12}(b_{21}c_{12} + b_{22}c_{22}) \\
a_{21}(b_{11}c_{11} + b_{12}c_{21}) + a_{22}(b_{21}c_{11} + b_{22}c_{21}) & a_{21}(b_{11}c_{12} + b_{12}c_{22}) + a_{22}(b_{21}c_{12} + b_{22}c_{22}) \\
\end{bmatrix}
\]
\[
=
\begin{bmatrix}
(a_{11}b_{11}+a_{12}b_{21})c_{11} +(a_{11}b_{12}+a_{12}b_{22})c_{21}& (a_{11}b_{11}+a_{12}b_{21})c_{12} +(a_{11}b_{12}+a_{12}b_{22})c_{22} \\
(a_{21}b_{11}+a_{22}b_{21})c_{11} +(a_{21}b_{12}+a_{22}b_{22})c_{21} & (a_{21}b_{11}+a_{22}b_{21})c_{12} +(a_{21}b_{12}+a_{22}b_{22})c_{22}\\
\end{bmatrix}
\]
$
= (AB)C  
$ \\For larger scale,maybe it's better to focus on only one element of the matrix.
\paragraph{Exercise 5.}
\[
A^2=
\begin{bmatrix}
    3 & 1\\
    1 & -3\\
\end{bmatrix}
\begin{bmatrix}
    3 & 1\\
    1 & -3\\
\end{bmatrix}
=
\begin{bmatrix}
    3 & 1\\
    1 & -3\\
\end{bmatrix}
=
\begin{bmatrix}
    10 & 0\\
    0 & 10\\
\end{bmatrix}
\]
\[
A^3=A^2*A=
\begin{bmatrix}
    10 & 0\\
    0 & 10\\
\end{bmatrix}
\begin{bmatrix}
    3 & 1\\
    1 & -3\\
\end{bmatrix}
=
\begin{bmatrix}
    30 & 10\\
    10 & -30\\
\end{bmatrix}
\]
\[
A^4=A^3*A=
\begin{bmatrix}
    30 & 10\\
    10 & -30\\
\end{bmatrix}
\begin{bmatrix}
    3 & 1\\
    1 & -3\\
\end{bmatrix}
=
\begin{bmatrix}
    100 & 0\\
    0 & 100\\
\end{bmatrix}
\]
\[...\]
Following the pattern $A^{2n}=
\begin{bmatrix}
    10^n & 0\\
    0 & 10^n\\
\end{bmatrix}
(n\in N)
$\\
\[A^{50}=
\begin{bmatrix}
    10^{25} & 0\\
    0 & 10^{25}\\
\end{bmatrix}
,A^{51}=
\begin{bmatrix}
    3*10^{25} & 10^{25}\\
    10^{25} & -3*10^{25}\\
\end{bmatrix}
\]
\end{document}
